theories/logrel/ftlr_nop.v
@@ -11,8 +11,9 @@ Section ftlr_nop.
   Context `{hypparams:!HypervisorParameters}.
   Context `{vmG: !gen_VMG Σ}.
 
-Lemma ftlr_nop {i mem_acc_tx ai regs ps_acc p_tx p_rx instr} trans rx_state:
+Lemma ftlr_nop {i mem_acc_tx ai regs rxs rs ps_acc p_tx p_rx instr} trans:
   base_extra.is_total_gmap regs ->
+  base_extra.is_total_gmap rxs ->
   {[p_tx; p_rx]} ⊆ ps_acc ->
   currently_accessible_in_trans_memory_pages i trans ⊆ ps_acc ∖ {[p_tx; p_rx]} ->
   p_rx ∉ ps_acc ∖ {[p_rx; p_tx]} ∪ accessible_in_trans_memory_pages i trans ->
@@ -41,13 +42,13 @@ Lemma ftlr_nop {i mem_acc_tx ai regs ps_acc p_tx p_rx instr} trans rx_state:
               R0 @@ V0 ->r encode_hvc_func Run -∗
               R1 @@ V0 ->r encode_vmid i -∗
               (∃ r2 : Addr, R2 @@ V0 ->r r2) -∗
-              RX_state@i:= a2 -∗
               mailbox.rx_page i p_rx -∗
-              rx_pages (list_to_set list_of_vmids ∖ {[i]}) -∗
-              ▷ VMProp V0 (vmprop_zero i p_tx p_rx) (1 / 2) -∗
+              rx_states_global (delete i rxs) -∗
+              ▷ VMProp V0 (vmprop_zero i p_tx p_rx rxs) (1 / 2) -∗
               VMProp i (vmprop_unknown i p_tx p_rx) 1 -∗
               transaction_pagetable_entries_owned i a1 -∗
               retrieved_transaction_owned i a1 -∗
+              RX_state@i := a2 -∗
               (∃ mem : lang.mem, memory_pages (a0 ∪ (accessible_in_trans_memory_pages i a1)) mem) -∗
               WP ExecI @ i {{ _, True }}) -∗
    ([∗ map] r↦w ∈ regs, r @@ i ->r w) -∗
@@ -61,10 +62,10 @@ Lemma ftlr_nop {i mem_acc_tx ai regs ps_acc p_tx p_rx instr} trans rx_state:
    R0 @@ V0 ->r encode_hvc_func Run -∗
    R1 @@ V0 ->r encode_vmid i -∗
    (∃ r2 : Addr, R2 @@ V0 ->r r2) -∗
-   RX_state@i:= rx_state -∗
+   RX_state@i:= rs -∗
    mailbox.rx_page i p_rx -∗
-   rx_pages (list_to_set list_of_vmids ∖ {[i]}) -∗
-   ▷ VMProp V0 (vmprop_zero i p_tx p_rx) (1 / 2) -∗
+   rx_states_global (delete i rxs) -∗
+   ▷ VMProp V0 (vmprop_zero i p_tx p_rx rxs) (1 / 2) -∗
    VMProp i (vmprop_unknown i p_tx p_rx) 1 -∗
    transaction_pagetable_entries_owned i trans -∗
    retrieved_transaction_owned i trans -∗
@@ -73,7 +74,7 @@ Lemma ftlr_nop {i mem_acc_tx ai regs ps_acc p_tx p_rx instr} trans rx_state:
    (∃ mem2 : mem, memory_page p_tx mem2) -∗
    SSWP ExecI @ i {{ bm, (if bm.1 then VMProp_holds i (1 / 2) else True) -∗ WP bm.2 @ i {{ _, True }} }}.
   Proof.
-    iIntros (Htotal_regs Hsubset_mb Hsubset_acc Hnin_rx Hnin_tx Hlookup_PC Hin_ps_acc Hneq_ptx Hdom_mem_acc_tx Hin_ps_acc_tx Hlookup_mem_ai Heqn).
+    iIntros (Htotal_rxs Htotal_regs Hsubset_mb Hsubset_acc Hnin_rx Hnin_tx Hlookup_PC Hin_ps_acc Hneq_ptx Hdom_mem_acc_tx Hin_ps_acc_tx Hlookup_mem_ai Heqn).
     iIntros "IH regs tx pgt_tx pgt_acc pgt_owned trans_hpool_global tran_pgt_transferred retri R0z R1z R2z rx_state rx other_rx prop0 propi tran_pgt_owned
                  retri_owned mem_rest mem_acc_tx mem_tx".
     (* getting the PC *)
@@ -89,8 +90,8 @@ Lemma ftlr_nop {i mem_acc_tx ai regs ps_acc p_tx p_rx instr} trans rx_state:
     iDestruct ("Hacc_regs" $! (ai ^+ 1)%f with "PC") as "[%Htotal_regs' regs]".
     iDestruct ("Hacc_mem_acc" with "[$mem_instr]") as "mem_acc_tx".
     iApply ("IH" $! _ ps_acc trans _ Htotal_regs' Hsubset_mb Hsubset_acc Hnin_rx Hnin_tx with "regs tx pgt_tx pgt_acc pgt_owned
-                       trans_hpool_global tran_pgt_transferred retri R0z R1z R2z rx_state rx other_rx prop0 propi
-                           tran_pgt_owned retri_owned [mem_rest mem_acc_tx mem_tx]").
+                       trans_hpool_global tran_pgt_transferred retri R0z R1z R2z rx other_rx prop0 propi
+                           tran_pgt_owned retri_owned rx_state [mem_rest mem_acc_tx mem_tx]").
     {
       iDestruct (memory_pages_split_singleton' p_tx ps_acc with "[mem_acc_tx $mem_tx]") as "mem_acc". set_solver + Hsubset_mb.
       iExists mem_acc_tx;by iFrame "mem_acc_tx".
